\documentclass{article}

\usepackage{enumerate}
\usepackage{amsmath}
\usepackage{color}

\begin{document}

% the preamble
\title{BIOST 311: \\ Interpreting coefficients after transformations}
\author{Kelsey Grinde and Brian Williamson}
\date{Spring 2018}

% title
\maketitle

\section{Transformations of the predictor}

Interpret $\beta_0, \beta_1$ in the following models:

\begin{enumerate}\itemsep +5pt
\item $E[\text{FEV}|\left(\text{Age}-\overline{Age}\right)] = \beta_0 + \beta_1 \left(\text{Age}-\overline{Age}\right)$ 
\item[] \color{blue} \textbf{Answer:} \\
% beta_0
$\beta_0$: average FEV (l/sec) among subjects with average (in the dataset) age \\
\begin{align*}
E[\text{FEV}|\text{Age} = \overline{Age}] &= E[\text{FEV}|\left(\text{Age}-\overline{Age}\right)=\overline{Age}-\overline{Age}]\\
& = E[\text{FEV}|\left(\text{Age}-\overline{Age}\right) =0]\\
& = \beta_0+ \beta_1(0) \\
& = \beta_0
\end{align*}
% beta_1
$\beta_1$: difference in average FEV (l/sec) comparing two groups that differ in age by one year
\begin{align*}
&E[\text{FEV}|\text{Age} = x + 1] - E[\text{FEV}|\text{Age} = x ] \\
&=E[\text{FEV}|\left(\text{Age}-\overline{Age}\right)= x + 1 - \overline{Age}] - E[\text{FEV}|\left(\text{Age}-\overline{Age}\right)= x  - \overline{Age}]\\
&=\left[\beta_0 + \beta_1\left( x + 1 - \overline{Age}\right)\right] - \left[\beta_0 + \beta_1\left( x  - \overline{Age}\right)\right] \\
&=\left[\beta_0 + \beta_1(x) + \beta_1 (1)  +\beta_1(-\overline{Age})\right] -\left[\beta_0 + \beta_1(x)  +\beta_1(-\overline{Age})\right]\\
& = \beta_1
\end{align*}
\color{black}

\newpage
\item $E[\text{FEV}|\left(\frac{\text{Age}}{10}\right)] = \beta_0 + \beta_1 \left(\frac{\text{Age}}{10}\right)$ 
\item[] \color{blue} \textbf{Answer:} \\
% beta_0
$\beta_0$: average FEV (l/sec) among newborns \\
\begin{align*}
E[\text{FEV}|\text{Age} =0] &= E[\text{FEV}|\left(\frac{\text{Age}}{10}\right)=\left(\frac{0}{10}\right)]\\
& = E[\text{FEV}|\left(\frac{\text{Age}}{10}\right) =0]\\
& = \beta_0+ \beta_1(0) \\
& = \beta_0
\end{align*}
% beta_1
$\beta_1$: difference in average FEV (l/sec) comparing two groups that differ in age by one decade (10 years)
\begin{align*}
&E[\text{FEV}|\text{Age} = x + 10] - E[\text{FEV}|\text{Age} = x ] \\
&=E[\text{FEV}|\left(\frac{\text{Age}}{10}\right)= \left(\frac{x+10}{10}\right)] - E[\text{FEV}|\left(\frac{\text{Age}}{10}\right)= \left(\frac{x}{10}\right)]\\
&=\left[\beta_0 + \beta_1\left(\frac{x+10}{10}\right)\right] - \left[\beta_0 + \beta_1\left(\frac{x}{10}\right)\right] \\
&=\left[\beta_0 + \beta_1\left(\frac{x}{10}\right) + \beta_1\left(\frac{10}{10}\right)\right] -\left[\beta_0 + \beta_1\left(\frac{x}{10}\right) \right]\\
& = \beta_1
\end{align*}
\color{black}

\newpage
\item $E[\text{FEV}|\left(\frac{\text{Age}-3}{10}\right)] = \beta_0 + \beta_1 \left(\frac{\text{Age}-3}{10}\right)$ 
\item[] \color{blue} \textbf{Answer:} 
% beta_0
$\beta_0$: average FEV (l/sec) among 3 year olds \\
\begin{align*}
E[\text{FEV}|\text{Age} =3] &= E[\text{FEV}|\left(\frac{\text{Age}-3}{10}\right)=\left(\frac{3-3}{10}\right)]\\
& = E[\text{FEV}|\left(\frac{\text{Age}-3}{10}\right) =0]\\
& = \beta_0+ \beta_1(0) \\
& = \beta_0
\end{align*}
% beta_1
$\beta_1$: difference in average FEV (l/sec) comparing two groups that differ in age by one decade (10 years)
\begin{align*}
&E[\text{FEV}|\text{Age} = x + 10] - E[\text{FEV}|\text{Age} = x ] \\
&=E[\text{FEV}|\left(\frac{\text{Age}-3}{10}\right)= \left(\frac{x+10-3}{10}\right)] - E[\text{FEV}|\left(\frac{\text{Age}-3}{10}\right)= \left(\frac{x-3}{10}\right)]\\
&=\left[\beta_0 + \beta_1\left(\frac{x+10-3}{10}\right)\right] - \left[\beta_0 + \beta_1\left(\frac{x-3}{10}\right)\right] \\
&=\left[\beta_0 + \beta_1\left(\frac{x-3}{10}\right) + \beta_1\left(\frac{10}{10}\right)\right] -\left[\beta_0 + \beta_1\left(\frac{x-3}{10}\right) \right]\\
& = \beta_1
\end{align*}
\color{black}
\end{enumerate}

% transforming the outcome
\newpage
\section{Transformations of the outcome}
Interpret $\beta_0, \beta_1$ in the following models:
\begin{enumerate}\itemsep +5pt
\item $E[(\text{FEV}\times 60)|\text{Age}] = \beta_0 + \beta_1 \text{Age}$ 
\item[] \color{blue} \textbf{Answer:} \\
% units
By multiplying FEV by 60, we've changed the units from l/sec to l/min:
\begin{align*}
\text{FEV}\frac{\text{liters}}{\text{sec}} & =\frac{\text{FEV liters}}{\text{sec}} \times \frac{60 \text{ sec}}{1\text{ min}} \\
& = (\text{FEV} \times 60) \frac{\text{ liters}}{\text{min}}\\
\text{Example: } 30\frac{\text{liters}}{\text{sec}} &= 180\frac{\text{liters}}{\text{min}}
\end{align*}
Then, the rest of our interpretation is the same as without the transformation, except we have new units...\\ \\
% beta_0
$\beta_0$: average FEV (l/min) among newborns \\
\begin{align*}
E[(\text{FEV}\times 60)|\text{Age} = 0] & = \beta_0+ \beta_1(0) \\
& = \beta_0 \\
\end{align*}
% beta_1
$\beta_1$: difference in average FEV (l/min) comparing two groups that differ in age by one year
\begin{align*}
&E[(\text{FEV}\times 60)|\text{Age} = x + 1] - E(\text{FEV}\times 60)|\text{Age} = x ] \\
&=\left[\beta_0 + \beta_1\left( x + 1\right)\right] - \left[\beta_0 + \beta_1\left( x \right)\right] \\
&=\left[\beta_0 + \beta_1(x) + \beta_1 (1)\right] -\left[\beta_0 + \beta_1(x)\right]\\
& = \beta_1
\end{align*}
\color{black}

\newpage
\item $E[\left(\frac{\text{FEV}}{3.78541}\right)|\text{Age}] = \beta_0 + \beta_1 \text{Age}$ \begin{scriptsize}(Hint: 1 gallon = 3.78541 liters)\end{scriptsize}
\item[] \color{blue} \textbf{Answer:} \\
% units
By dividing FEV by 3.78541, we've changed the units from l/sec to gal/sec:
\begin{align*}
\text{FEV}\frac{\text{liters}}{\text{sec}} & =\frac{\text{FEV liters}}{\text{sec}} \times \frac{1\text{ gallon}}{ 3.78541\text{ liters}} \\ 
& = (\text{FEV} \div 3.78541) \frac{\text{gallons}}{\text{sec}}\\
\text{Example: } 30\frac{\text{liters}}{\text{sec}} &= 7.925\frac{\text{gallons}}{\text{sec}}
\end{align*}
Then, the rest of our interpretation is the same as without the transformation, except we have new units...\\ \\
% beta_0
$\beta_0$: average FEV (gal/sec) among newborns \\
\begin{align*}
E[(\text{FEV}\times 60)|\text{Age} = 0] & = \beta_0+ \beta_1(0) \\
& = \beta_0 \\
\end{align*}
% beta_1
$\beta_1$: difference in average FEV (gal/sec) comparing two groups that differ in age by one year
\begin{align*}
&E[(\text{FEV}\div 3.78541 )|\text{Age} = x + 1] - E(\text{FEV}\div 3.78541 )|\text{Age} = x ] \\
&=\left[\beta_0 + \beta_1\left( x + 1\right)\right] - \left[\beta_0 + \beta_1\left( x \right)\right] \\
&=\left[\beta_0 + \beta_1(x) + \beta_1 (1)\right] -\left[\beta_0 + \beta_1(x)\right]\\
& = \beta_1
\end{align*}
\color{black}
\end{enumerate}


\end{document}
